thesis example and some clean up

Cdclt/Lift/Defs.lean
@@ -1,4 +1,5 @@
 import Cdclt.Lift.Env
+import Cdclt.Lift.Utils
 import Cdclt.Lift.Types
 import Cdclt.Lift.Coe
 import Cdclt.Term
@@ -10,51 +11,53 @@ open sort
 
 set_option maxHeartbeats 500000
 
-def falseInterp : Interpretation := ⟨boolSort, λ Γ Δ => False⟩
-
 @[simp] def combineProps : Interpretation → Interpretation → (Prop → Prop → Prop) → Interpretation
-| ⟨ boolSort, k₁ ⟩, ⟨ boolSort, k₂ ⟩, f =>
-    ⟨ boolSort, λ Δ Γ => f (k₁ Δ Γ) (k₂ Δ Γ) ⟩
-| _, _, _ => falseInterp
+| some ⟨ boolSort, k₁ ⟩, some ⟨ boolSort, k₂ ⟩, f =>
+    some ⟨ boolSort, λ Γ Δ => f (k₁ Γ Δ) (k₂ Γ Δ) ⟩ -- maybe we can use state monad to avoid propagating the environments manually?
+| _, _, _ => none
 
 @[simp] def interpTerm : term → Interpretation
-| term.const   n  s  => ⟨ s, λ _ Γ => Γ s n  ⟩
+| term.const   n  s  => some ⟨ s, λ Γ Δ => Γ n Δ s  ⟩
 | term.not     t₁    => match interpTerm t₁ with
-                        | ⟨ boolSort, k ⟩ => ⟨ boolSort, λ Δ Γ => ¬ (k Δ Γ) ⟩
-                        | _ => falseInterp
+                        | some ⟨ boolSort, k ⟩ => some ⟨ boolSort, λ Γ Δ => ¬ (k Γ Δ) ⟩
+                        | _ => none
 | term.and     t₁ t₂ => combineProps (interpTerm t₁) (interpTerm t₂) (λ p₁ p₂ => p₁ ∧ p₂)
 | term.or      t₁ t₂ => combineProps (interpTerm t₁) (interpTerm t₂) (λ p₁ p₂ => p₁ ∨ p₂)
 | term.implies t₁ t₂ => combineProps (interpTerm t₁) (interpTerm t₂) (λ p₁ p₂ => p₁ → p₂)
 | term.xor     t₁ t₂ => combineProps (interpTerm t₁) (interpTerm t₂) (λ p₁ p₂ => p₁ ≠ p₂)
+/- | term.eq      t₁ t₂ => combineProps (interpTerm t₁) (interpTerm t₂) (λ p₁ p₂ => p₁ = p₂) -/
 | term.eq      t₁ t₂ => match interpTerm t₁, interpTerm t₂ with
-                        | ⟨ s₁, k₁ ⟩, ⟨ s₂, k₂ ⟩ =>
+                        | some ⟨ s₁, k₁ ⟩, some ⟨ s₂, k₂ ⟩ =>
                           if r: s₂ = s₁
-                          then ⟨ boolSort, λ Δ Γ =>
+                          then some ⟨ boolSort, λ Γ Δ =>
                                             let coercion := coe' (congrArg (interpSort Δ) r) 
-                                            k₁ Δ Γ = coercion (k₂ Δ Γ) ⟩
-                          else falseInterp
-| term.bot           => ⟨ boolSort, λ _ _ => False ⟩
-| term.top           => ⟨ boolSort, λ _ _ => True  ⟩
+                                            k₁ Γ Δ = coercion (k₂ Γ Δ) ⟩
+                          else none
+                        | _, _ => none
+| term.bot           => some ⟨ boolSort, λ _ _ => False ⟩
+| term.top           => some ⟨ boolSort, λ _ _ => True  ⟩
 | term.app     t₁ t₂ => match interpTerm t₁, interpTerm t₂ with
-                        | ⟨ arrow s₁₁ s₁₂, k₁ ⟩, ⟨ s₂, k₂ ⟩ =>
+                        | some ⟨ arrow s₁₁ s₁₂, k₁ ⟩, some ⟨ s₂, k₂ ⟩ =>
                           if r: s₂ = s₁₁
-                          then ⟨ s₁₂ , λ Δ Γ =>
+                          then some ⟨ s₁₂ , λ Γ Δ =>
                                               let coercion := coe' (congrArg (interpSort Δ) r)
-                                              k₁ Δ Γ (coercion (k₂ Δ Γ)) ⟩
-                          else falseInterp
-                        | _, _ => falseInterp
-| _ => falseInterp
+                                              k₁ Γ Δ (coercion (k₂ Γ Δ)) ⟩
+                          else none
+                        | _, _ => none
+| _ => none
 
-@[simp] def validWith (Δ : SEnvironment) (Γ : Environment Δ) (t : term) : Prop :=
+@[simp] def validWith (Γ : Environment) (Δ : SEnvironment) (t : term) : Prop :=
   match interpTerm t with
-  | ⟨ boolSort, k ⟩ => Coe.coe (k Δ Γ)
+  | some ⟨ boolSort, k ⟩ => Coe.coe (k Γ Δ)
   | _ => False
 
 def followsFrom (t₁ t₂ : term) : Prop :=
-  ∀ {Δ : SEnvironment} {Γ : Environment Δ}, validWith Δ Γ t₁ → validWith Δ Γ t₂
+  ∀ {Γ : Environment} {Δ : SEnvironment}, validWith Γ Δ t₁ → validWith Γ Δ t₂
 
-/- @[simp] def getInterp (t : term) (h : wellTyped t) : Σ (s : sort), Environment → (Δ : SEnvironment) → interpSort Δ s := -/
-/-   match r: interpTerm t with -/
-/-   | some ⟨ s, k ⟩ => ⟨ s, k ⟩ -/
-/-   | none => by simp at h; rewrite [r] at h; exact (False.elim h) -/
+@[simp] def wellTyped (t : term) : Prop := isSome (interpTerm t)
+
+@[simp] def getInterp (t : term) (h : wellTyped t) : Σ (s : sort), Environment → (Δ : SEnvironment) → interpSort Δ s :=
+  match r: interpTerm t with
+  | some ⟨ s, k ⟩ => ⟨ s, k ⟩
+  | none => by simp at h; rewrite [r] at h; exact (False.elim h)
 
