Cdclt/Lift/ThesisExample.lean
@@ -1,0 +1,342 @@
+import Cdclt.Term
+import Cdclt.Boolean
+
+open proof
+open sort
+open term
+
+/- -- Auxiliary -/
+
+theorem eqTrue {A : Prop} : A = True → A := fun ha => by rw [ha]; exact True.intro
+
+theorem eqFalse {A : Prop} : A = False → ¬ A := fun hna => by rw [hna]; simp
+
+theorem impliesEqTrue {A : Prop} : A → (A = True) := fun ha =>
+  propext $ Iff.intro (fun _ => True.intro) (fun _ => ha)
+
+theorem impliesEqFalse {A : Prop} : ¬ A → (A = False) := fun hna =>
+  propext $ Iff.intro (fun ha => hna ha) False.elim
+
+theorem negNegElim {A : Prop} : ¬ ¬ A → A := by
+  cases Classical.em A with
+  | inl c => exact fun _ => c
+  | inr c => exact fun h => False.elim (h c)
+
+def coe' : (A = B) → A → B
+| rfl, a => a
+
+/- -- Definitions -/
+
+def interpSort' : sort → Type := fun s =>
+  match s with
+  | sort.arrow s₁ s₂ => interpSort' s₁ → interpSort' s₂
+  | boolSort => Prop
+  | _ => Prop
+
+def Interpretation : Type := Nat → Option (Σ (s : sort) , interpSort' s)
+
+@[simp] def evalTerm (I : Interpretation) (t : term) : Option (Σ (s : sort) , interpSort' s) :=
+  match t with
+  | term.const   i  _  => I i
+  | term.not     t₁    =>
+    match evalTerm I t₁ with
+    | some ⟨ boolSort, t₁' ⟩ => some ⟨ boolSort, ¬ t₁' ⟩
+    | _ => none
+  | term.and     t₁ t₂ =>
+    match evalTerm I t₁, evalTerm I t₂ with
+    | some ⟨ boolSort, t₁'⟩, some ⟨ boolSort , t₂' ⟩ => some ⟨ boolSort, And t₁' t₂' ⟩
+    | _,_ => none
+  | term.or      t₁ t₂ =>
+    match evalTerm I t₁, evalTerm I t₂ with
+    | some ⟨ boolSort, t₁'⟩, some ⟨ boolSort , t₂' ⟩ => some ⟨ boolSort, Or t₁' t₂' ⟩
+    | _,_ => none
+  | term.implies t₁ t₂ =>
+    match evalTerm I t₁, evalTerm I t₂ with
+    | some ⟨ boolSort, t₁'⟩, some ⟨ boolSort , t₂' ⟩ => some ⟨ boolSort, t₁' → t₂' ⟩
+    | _,_ => none
+  | term.eq      t₁ t₂ =>
+    match evalTerm I t₁, evalTerm I t₂ with
+    | some ⟨ s₁, t₁'⟩, some ⟨ s₂, t₂' ⟩ =>
+      if r: s₁ = s₂ then
+        let ct₂' := coe' (congrArg interpSort' (Eq.symm r)) t₂'
+        some ⟨ boolSort, t₁' = ct₂' ⟩
+      else none
+    | _,_ => none
+  | term.bot           => some ⟨ boolSort, False ⟩
+  | term.top           => some ⟨ boolSort, True ⟩
+  | _                  => none
+
+@[simp] def satisfies (I : Interpretation) (t : term) : Prop :=
+  match evalTerm I t with
+  | some ⟨ boolSort, p ⟩ => p = True
+  | _ => False
+
+def impliesIn (t₁ t₂ : term) : Prop :=
+  ∀ {I : Interpretation}, satisfies I t₁ → satisfies I t₂
+
+theorem notImplies1 : ∀ {t₁ t₂ : term},
+    impliesIn (not (implies t₁ t₂)) t₁ := by
+  intros t₁ t₂
+  rw [impliesIn]
+  intros I h
+  simp at h
+  split at h
+  case h_1 _ _ h' =>
+    split at h'
+    case h_1 _ d h'' =>
+      split at h''
+      case h_1 h₃ _ f _ i _ =>
+        injection h'' with h''
+        injection h'' with _ h''
+        injection h' with h'
+        injection h' with _ h'
+        rw [satisfies, i]
+        rw [h] at h'
+        have hh : d = False := impliesEqFalse (eqTrue h')
+        rw [hh] at h''
+        have z := eqFalse h''
+        apply impliesEqTrue
+        cases Classical.em f with
+        | inl c => exact c
+        | inr c => exact False.elim (z (fun hf   => False.elim (c hf)))
+      case h_2 a b h₃                            => injection h''
+    case h_2 h''                                 => injection h'
+  case h_2 hh                                    => exact False.elim h
+
+open Nat
+
+theorem notImplies2 : ∀ {t₁ t₂ : term},
+    impliesIn (not $ implies t₁ t₂) (not t₂) := by
+  intros t₁ t₂
+  rw [impliesIn]
+  intros I h
+  simp at h
+  match r₁: evalTerm I t₁, r₂: evalTerm I t₂ with
+  | some ⟨ boolSort, p₁ ⟩, some ⟨ boolSort, p₂ ⟩ =>
+    rw [r₁, r₂] at h
+    have h₂ : (¬ ( p₁ → p₂ ))                    = True := h
+    rw [satisfies]
+    simp
+    rw [r₂]
+    show (¬ p₂) = True
+    apply impliesEqTrue
+    intro hp₂
+    have h₂' := eqTrue h₂
+    exact (h₂' (fun hp₁ => hp₂))
+  | some ⟨ atom 0, _ ⟩, _                                => rw [r₁] at h; cases h
+  | some ⟨ atom 1, _ ⟩, some ⟨ atom 0, _ ⟩               => rw [r₁, r₂] at h; cases h
+  | some ⟨ atom 1, _ ⟩, some ⟨ atom (succ (succ _)), _ ⟩ => rw [r₁, r₂] at h; cases h
+  | some ⟨ atom 1, _ ⟩, some ⟨ sort.undef, _ ⟩           => rw [r₁, r₂] at h; cases h
+  | some ⟨ atom 1, _ ⟩, some ⟨ sort.array _ _, _ ⟩       => rw [r₁, r₂] at h; cases h
+  | some ⟨ atom 1, _ ⟩, some ⟨ sort.bv _, _ ⟩            => rw [r₁, r₂] at h; cases h
+  | some ⟨ atom 1, _ ⟩, some ⟨ sort.arrow _ _, _ ⟩       => rw [r₁, r₂] at h; cases h
+  | some ⟨ atom 1, _ ⟩, some ⟨ sort.dep, _ ⟩             => rw [r₁, r₂] at h; cases h
+  | some ⟨ atom 1, _ ⟩, none                             => rw [r₁, r₂] at h; cases h
+  | some ⟨ atom (succ (succ _)), _ ⟩, _                  => rw [r₁] at h; cases h
+  | some ⟨ sort.undef, _ ⟩, _                            => rw [r₁] at h; cases h
+  | some ⟨ sort.array _ _, _ ⟩, _                        => rw [r₁] at h; cases h
+  | some ⟨ sort.bv _, _ ⟩, _                             => rw [r₁] at h; cases h
+  | some ⟨ sort.arrow _ _, _ ⟩, _                        => rw [r₁] at h; cases h
+  | some ⟨ sort.dep, _ ⟩, _                              => rw [r₁] at h; cases h
+  | none, _                                              => rw [r₁] at h; cases h
+
+theorem impliesElim : ∀ {t₁ t₂ : term},
+    impliesIn (implies t₁ t₂) (or (not t₁) t₂) := by
+  intros t₁ t₂
+  rw [impliesIn]
+  intros I h
+  simp at h
+  match r₁: evalTerm I t₁, r₂: evalTerm I t₂ with
+  | some ⟨ boolSort, p₁ ⟩, some ⟨ boolSort, p₂ ⟩ =>
+    rw [r₁, r₂] at h
+    have h₂ : ( p₁ → p₂ ) = True := h
+    rw [satisfies]
+    simp
+    rw [r₁, r₂]
+    show (¬ p₁ ∨ p₂) = True
+    apply impliesEqTrue
+    have h₂' := eqTrue h₂
+    cases Classical.em p₁ with
+    | inl c => exact Or.inr (h₂' c)
+    | inr c => exact Or.inl c
+  | some ⟨ atom 0, _ ⟩, _                                => rw [r₁] at h; cases h
+  | some ⟨ atom 1, _ ⟩, some ⟨ atom 0, _ ⟩               => rw [r₁, r₂] at h; cases h
+  | some ⟨ atom 1, _ ⟩, some ⟨ atom (succ (succ _)), _ ⟩ => rw [r₁, r₂] at h; cases h
+  | some ⟨ atom 1, _ ⟩, some ⟨ sort.undef, _ ⟩           => rw [r₁, r₂] at h; cases h
+  | some ⟨ atom 1, _ ⟩, some ⟨ sort.array _ _, _ ⟩       => rw [r₁, r₂] at h; cases h
+  | some ⟨ atom 1, _ ⟩, some ⟨ sort.bv _, _ ⟩            => rw [r₁, r₂] at h; cases h
+  | some ⟨ atom 1, _ ⟩, some ⟨ sort.arrow _ _, _ ⟩       => rw [r₁, r₂] at h; cases h
+  | some ⟨ atom 1, _ ⟩, some ⟨ sort.dep, _ ⟩             => rw [r₁, r₂] at h; cases h
+  | some ⟨ atom 1, _ ⟩, none                             => rw [r₁, r₂] at h; cases h
+  | some ⟨ atom (succ (succ _)), _ ⟩, _                  => rw [r₁] at h; cases h
+  | some ⟨ sort.undef, _ ⟩, _                            => rw [r₁] at h; cases h
+  | some ⟨ sort.array _ _, _ ⟩, _                        => rw [r₁] at h; cases h
+  | some ⟨ sort.bv _, _ ⟩, _                             => rw [r₁] at h; cases h
+  | some ⟨ sort.arrow _ _, _ ⟩, _                        => rw [r₁] at h; cases h
+  | some ⟨ sort.dep, _ ⟩, _                              => rw [r₁] at h; cases h
+  | none, _                                              => rw [r₁] at h; cases h
+
+theorem R1 : ∀ {t₁ t₂ : term},
+    impliesIn (and (or (not t₁) t₂) t₁) t₂ := by
+  intros t₁ t₂
+  rw [impliesIn]
+  intros I h
+  simp at h
+  match r₁: evalTerm I t₁, r₂: evalTerm I t₂ with
+  | some ⟨ boolSort, p₁ ⟩, some ⟨ boolSort, p₂ ⟩ =>
+    rw [r₁, r₂] at h
+    have h₂ : (((¬ p₁) ∨ p₂) ∧ p₁) = True := h
+    rw [satisfies]
+    simp
+    rw [r₂]
+    show p₂ = True
+    apply impliesEqTrue
+    have h₂' := eqTrue h₂
+    have ⟨hOr, hp₁⟩ := h₂'
+    cases hOr with
+    | inl hnp₁ => exact False.elim (hnp₁ hp₁) 
+    | inr hp₂  => exact hp₂
+  | some ⟨ atom 0, _ ⟩, _                                => rw [r₁] at h; cases h
+  | some ⟨ atom 1, _ ⟩, some ⟨ atom 0, _ ⟩               => rw [r₁, r₂] at h; cases h
+  | some ⟨ atom 1, _ ⟩, some ⟨ atom (succ (succ _)), _ ⟩ => rw [r₁, r₂] at h; cases h
+  | some ⟨ atom 1, _ ⟩, some ⟨ sort.undef, _ ⟩           => rw [r₁, r₂] at h; cases h
+  | some ⟨ atom 1, _ ⟩, some ⟨ sort.array _ _, _ ⟩       => rw [r₁, r₂] at h; cases h
+  | some ⟨ atom 1, _ ⟩, some ⟨ sort.bv _, _ ⟩            => rw [r₁, r₂] at h; cases h
+  | some ⟨ atom 1, _ ⟩, some ⟨ sort.arrow _ _, _ ⟩       => rw [r₁, r₂] at h; cases h
+  | some ⟨ atom 1, _ ⟩, some ⟨ sort.dep, _ ⟩             => rw [r₁, r₂] at h; cases h
+  | some ⟨ atom 1, _ ⟩, none                             => rw [r₁, r₂] at h; cases h
+  | some ⟨ atom (succ (succ _)), _ ⟩, _                  => rw [r₁] at h; cases h
+  | some ⟨ sort.undef, _ ⟩, _                            => rw [r₁] at h; cases h
+  | some ⟨ sort.array _ _, _ ⟩, _                        => rw [r₁] at h; cases h
+  | some ⟨ sort.bv _, _ ⟩, _                             => rw [r₁] at h; cases h
+  | some ⟨ sort.arrow _ _, _ ⟩, _                        => rw [r₁] at h; cases h
+  | some ⟨ sort.dep, _ ⟩, _                              => rw [r₁] at h; cases h
+  | none, _                                              => rw [r₁] at h; cases h
+
+theorem conjunction : ∀ {t₁ t₂ : term} {I : Interpretation},
+    satisfies I t₁ → satisfies I t₂ → satisfies I (and t₁ t₂) := by
+  intros t₁ t₂ I h₁ h₂
+  simp at *
+  match r₁: evalTerm I t₁, r₂: evalTerm I t₂ with
+  | some ⟨ boolSort, p₁ ⟩, some ⟨ boolSort, p₂ ⟩ =>
+    rw [r₁] at h₁
+    rw [r₂] at h₂
+    have h₁' : p₁ = True := h₁
+    have h₂' : p₂ = True := h₂
+    show (p₁ ∧ p₂) = True
+    apply impliesEqTrue
+    have h₁'' := eqTrue h₁'
+    have h₂'' := eqTrue h₂'
+    exact And.intro h₁'' h₂''
+  | some ⟨ atom 0, _ ⟩, _                                => rw [r₁] at h₁; cases h₁
+  | some ⟨ atom 1, _ ⟩, some ⟨ atom 0, _ ⟩               => rw [r₂] at h₂; cases h₂
+  | some ⟨ atom 1, _ ⟩, some ⟨ atom (succ (succ _)), _ ⟩ => rw [r₂] at h₂; cases h₂
+  | some ⟨ atom 1, _ ⟩, some ⟨ sort.undef, _ ⟩           => rw [r₂] at h₂; cases h₂
+  | some ⟨ atom 1, _ ⟩, some ⟨ sort.array _ _, _ ⟩       => rw [r₂] at h₂; cases h₂
+  | some ⟨ atom 1, _ ⟩, some ⟨ sort.bv _, _ ⟩            => rw [r₂] at h₂; cases h₂
+  | some ⟨ atom 1, _ ⟩, some ⟨ sort.arrow _ _, _ ⟩       => rw [r₂] at h₂; cases h₂
+  | some ⟨ atom 1, _ ⟩, some ⟨ sort.dep, _ ⟩             => rw [r₂] at h₂; cases h₂
+  | some ⟨ atom 1, _ ⟩, none                             => rw [r₂] at h₂; cases h₂
+  | some ⟨ atom (succ (succ _)), _ ⟩, _                  => rw [r₁] at h₁; cases h₁
+  | some ⟨ sort.undef, _ ⟩, _                            => rw [r₁] at h₁; cases h₁
+  | some ⟨ sort.array _ _, _ ⟩, _                        => rw [r₁] at h₁; cases h₁
+  | some ⟨ sort.bv _, _ ⟩, _                             => rw [r₁] at h₁; cases h₁
+  | some ⟨ sort.arrow _ _, _ ⟩, _                        => rw [r₁] at h₁; cases h₁
+  | some ⟨ sort.dep, _ ⟩, _                              => rw [r₁] at h₁; cases h₁
+  | none, _                                              => rw [r₁] at h₁; cases h₁
+
+theorem contradiction : ∀ {t : term},
+    impliesIn (and (not t) t) bot := by
+  intros t
+  rw [impliesIn]
+  intros I h
+  simp at *
+  show False = True
+  match r: evalTerm I t with
+  | some ⟨ boolSort, p ⟩ =>
+    rw [r] at h
+    have h' : (¬ p ∧ p) := eqTrue h
+    apply impliesEqTrue
+    have ⟨hnp, hp⟩ := h'
+    exact hnp hp
+  | some ⟨ atom 0, _ ⟩               => rw [r] at h; cases h
+  | some ⟨ atom (succ (succ _)), _ ⟩ => rw [r] at h; cases h
+  | some ⟨ sort.undef, _ ⟩           => rw [r] at h; cases h
+  | some ⟨ sort.array _ _, _ ⟩       => rw [r] at h; cases h
+  | some ⟨ sort.bv _, _ ⟩            => rw [r] at h; cases h
+  | some ⟨ sort.arrow _ _, _ ⟩       => rw [r] at h; cases h
+  | some ⟨ sort.dep, _ ⟩             => rw [r] at h; cases h
+  | none                             => rw [r] at h; cases h
+
+def p: term := const 1000 boolSort
+def q: term := const 1001 boolSort
+def modusPonensEmbed := implies p (implies (implies p q) q)
+def notModusPonensEmbed := not modusPonensEmbed
+
+theorem th0 : impliesIn notModusPonensEmbed bot :=
+  λ lean_a0 =>
+    have lean_s0 := notImplies2 lean_a0
+    have lean_s1 := notImplies1 lean_s0
+    have lean_s2 := impliesElim lean_s1
+    have lean_s4 := notImplies1 lean_a0
+    have lean_s6 := R1 (conjunction lean_s2 lean_s4)
+    have lean_s9 := notImplies2 lean_s0
+    contradiction (conjunction lean_s9 lean_s6)
+
+
+@[simp] def isBool (t : term) (I : Interpretation) : Bool :=
+  match evalTerm I t with
+  | some ⟨ boolSort, _ ⟩ => true
+  | _ => false
+
+theorem evalNotTerm: ∀ {I: Interpretation} {t: term},
+    isBool t I → ¬ satisfies I (not t)  → satisfies I t := by
+  intros I t bt h
+  simp [evalTerm] at h
+  match r: evalTerm I t with
+  | some ⟨ boolSort, p ⟩ =>
+    rw [r] at h
+    have h : ¬ ((¬ p) = True) := h
+    simp [satisfies]
+    rw [r]
+    show p = True
+    apply impliesEqTrue
+    cases Classical.em p with
+    | inl c => exact c
+    | inr c =>
+      have c' : (¬ p) = True := impliesEqTrue c
+      exact False.elim (h c') 
+  | some ⟨ atom 0, _ ⟩               => simp at bt; rw [r] at bt; cases bt
+  | some ⟨ atom (succ (succ _)), _ ⟩ => simp at bt; rw [r] at bt; cases bt
+  | some ⟨ sort.undef, _ ⟩           => simp at bt; rw [r] at bt; cases bt
+  | some ⟨ sort.array _ _, _ ⟩       => simp at bt; rw [r] at bt; cases bt
+  | some ⟨ sort.bv _, _ ⟩            => simp at bt; rw [r] at bt; cases bt
+  | some ⟨ sort.arrow _ _, _ ⟩       => simp at bt; rw [r] at bt; cases bt
+  | some ⟨ sort.dep, _ ⟩             => simp at bt; rw [r] at bt; cases bt
+  | none                             => simp at bt; rw [r] at bt; cases bt
+
+theorem impliesInBot : ∀ {t : term},
+    impliesIn t bot → ∀ {I : Interpretation}, ¬ satisfies I t := by
+  intros t h I
+  rw [impliesIn] at h
+  have h' := @h I
+  intro tSatisfied
+  have botSatisfied := h' tSatisfied
+  simp [satisfies] at botSatisfied
+  have abs : False = True := botSatisfied
+  simp at abs
+
+def modusPonens (P Q : Prop) : Prop := P → (P → Q) → Q
+
+theorem modusPonensCorrect: ∀ (P Q: Prop), (modusPonens P Q) = True := by
+  intros P Q
+  let I: Interpretation := fun id =>
+    if id == 1000 then
+      some ⟨ boolSort, P ⟩ 
+    else if id == 1001 then
+      some ⟨ boolSort, Q ⟩
+    else none
+  have mpBool : isBool modusPonensEmbed I := rfl
+  have f: ∀ {I' : Interpretation}, ¬ satisfies I' notModusPonensEmbed := impliesInBot th0
+  have notMpUnsatisfied : ¬ satisfies I notModusPonensEmbed := @f I
+  exact evalNotTerm mpBool notMpUnsatisfied
